AwsCryptographicMaterialProviders/dafny/AwsCryptographicMaterialProviders/src/KeyWrapping/IntermediateKeyWrapping.dfy
@@ -69,7 +69,9 @@ module IntermediateKeyWrapping {
           UnwrapInput(
             wrappedMaterial := maybeIntermediateWrappedMat.value.providerWrappedIkm,
             encryptionContext := encryptionContext,
-            algorithmSuite := algorithmSuite),
+            algorithmSuite := algorithmSuite,
+            serializedEC := CanonicalEncryptionContext.EncryptionContextToAAD(encryptionContext)
+          ),
           Success(unwrapRes),
           [])
 
@@ -82,12 +84,14 @@ module IntermediateKeyWrapping {
     // Deserialize the Intermediate-Wrapped material
     var deserializedWrapped :- DeserializeIntermediateWrappedMaterial(wrappedMaterial, algorithmSuite);
     var DeserializedIntermediateWrappedMaterial(encryptedPdk, providerWrappedIkm) := deserializedWrapped;
+    var serializedEC := CanonicalEncryptionContext.EncryptionContextToAAD(encryptionContext);
 
     var unwrapOutput :- unwrap.Invoke(
       UnwrapInput(
         wrappedMaterial := providerWrappedIkm,
         encryptionContext := encryptionContext,
-        algorithmSuite := algorithmSuite
+        algorithmSuite := algorithmSuite,
+        serializedEC := serializedEC
       ), []);
     var UnwrapOutput(intermediateMaterial, unwrapInfo) := unwrapOutput;
 
@@ -102,7 +106,7 @@ module IntermediateKeyWrapping {
     // Decrypt the plaintext data key with the pdkEncryptionKey
     var iv: seq<uint8> := seq(AlgorithmSuites.GetEncryptIvLength(algorithmSuite) as nat, _ => 0); // IV is zero
     var tagIndex := |encryptedPdk| - AlgorithmSuites.GetEncryptTagLength(algorithmSuite) as nat;
-    var aad :- CanonicalEncryptionContext.EncryptionContextToAAD(encryptionContext);
+    var aad :- serializedEC;
 
     var decInput := Crypto.AESDecryptInput(
       encAlg := algorithmSuite.encrypt.AES_GCM,
@@ -143,7 +147,9 @@ module IntermediateKeyWrapping {
         && generateAndWrap.Ensures(
              GenerateAndWrapInput(
                algorithmSuite := algorithmSuite,
-               encryptionContext := encryptionContext),
+               encryptionContext := encryptionContext,
+               serializedEC := CanonicalEncryptionContext.EncryptionContextToAAD(encryptionContext)
+             ),
              Success(
                GenerateAndWrapOutput(
                  plaintextMaterial := res.value.intermediateMaterial,
@@ -178,7 +184,8 @@ module IntermediateKeyWrapping {
     var generateAndWrapOutput :- generateAndWrap.Invoke(
       GenerateAndWrapInput(
         algorithmSuite := algorithmSuite,
-        encryptionContext := encryptionContext
+        encryptionContext := encryptionContext,
+        serializedEC := CanonicalEncryptionContext.EncryptionContextToAAD(encryptionContext)
       ), []);
 
     //= aws-encryption-sdk-specification/framework/algorithm-suites.md#intermediate-key-wrapping
@@ -213,7 +220,7 @@ module IntermediateKeyWrapping {
     var encryptedPdk :- encOutR.MapFailure(e => Types.AwsCryptographyPrimitives(e));
 
     assert |encryptedPdk.cipherText + encryptedPdk.authTag| ==
-            (AlgorithmSuites.GetEncryptKeyLength(algorithmSuite) + AlgorithmSuites.GetEncryptTagLength(algorithmSuite)) as nat;
+           (AlgorithmSuites.GetEncryptKeyLength(algorithmSuite) + AlgorithmSuites.GetEncryptTagLength(algorithmSuite)) as nat;
 
     var serializedMaterial := encryptedPdk.cipherText + encryptedPdk.authTag + providerWrappedIkm;
 
@@ -240,7 +247,8 @@ module IntermediateKeyWrapping {
         && maybeIntermediateWrappedMat.Success?
         && generateAndWrap.Ensures(GenerateAndWrapInput(
                                      algorithmSuite := algorithmSuite,
-                                     encryptionContext := encryptionContext
+                                     encryptionContext := encryptionContext,
+                                     serializedEC := CanonicalEncryptionContext.EncryptionContextToAAD(encryptionContext)
                                    ), Success(
                                      GenerateAndWrapOutput(
                                        plaintextMaterial := res.value.intermediateMaterial,
